\documentclass{article}
\usepackage{graphicx} % Required for inserting images
\usepackage{amsfonts,amssymb,amsmath,mathbbol,amsthm,amstext,esint,mathtools,nccmath,upgreek}
\graphicspath{ {./Images/} }
\setlength{\jot}{0.5cm}
\DeclareSymbolFontAlphabet{\mathbb}{AMSb}
\DeclareSymbolFontAlphabet{\mathbbl}{bbold}
\usepackage{graphics,graphicx,epsfig,ulem, xcolor, soul}
\usepackage[margin={2cm,2cm}]{geometry}
\usepackage{tikz,pgfplots}
\usepackage{siunitx}
\usepackage{multirow}
\usepackage{array}
\usepackage{physics, amsmath}
\usepackage{float}
\usepackage{cleveref}
\usepackage{booktabs}
\usepackage[american,siunitx]{circuitikz}
\usepackage{caption}
\usepackage{subcaption}
\usepackage{pgfplotstable}
\pgfplotsset{compat=1.3}
\renewcommand{\vec}[1]{\mathbf{#1}}
\let\oldhat\hat
\renewcommand{\hat}[1]{\oldhat{\mathbf{#1}}}
\AtBeginDocument{
\heavyrulewidth=.08em
\lightrulewidth=.05em
\cmidrulewidth=.03em
\belowrulesep=.65ex
\belowbottomsep=0pt
\aboverulesep=.4ex
\abovetopsep=0pt
\cmidrulesep=\doublerulesep
\cmidrulekern=.5em
\defaultaddspace=.5em
}


\begin{document}
\newpage
\begin{center}
       
       \vspace*{1cm}
        \LARGE
       \textbf{Assignment 2a}

       \vspace{0.5cm}
        PHYS4000
        Advanced Computational Quantum Mechanics
            
       \vspace{1.5cm}

       \text{Ryan Craft}\bigskip

       Unit Coordinated by\\
       Dr. Igor Bray
            
       \vspace{0.8cm}
     
            
       
       May 2023
            
\end{center}
\newpage



\section{Question 1}

Equation 2.17 is written as:

    \begin{gather}
        \frac{d^2u_l(r)}{dr^2} + 2(E+\frac{Z}{r}) u_l(r) = l(l+1)\frac{u_l(r)}{r^2}
    \end{gather}

    First we need to make $\rho$ the subject of the function which is done through the substitution of
    $\rho=kr$.

    \begin{gather}
        k^2 \frac{d^2u_l(\rho)}{d\rho^2} + 2(-\frac{k^2}{8}+\frac{Zk}{\rho})u_l(\rho) =  l(l+1)\frac{u_l(\rho)k^2}{\rho^2}
    \end{gather}

    Where we have substituted for $E$ by rearranging the definition of $k=2\sqrt{-2E}$. 
    We further simplify the differential Equation to the following by cancelling $k^2$ and multiplying the bracket:

    \begin{gather}
        \frac{d^2u_l(\rho)}{d\rho^2} - (\frac{1}{4}-\frac{2Z}{\rho k})u_l(\rho) =  l(l+1)\frac{u_l(\rho)}{\rho^2}
    \end{gather}

    In finding the solutions to the differential equation we rearrange it into the form\dots

    \begin{gather}
        \frac{d^2u_l(\rho)}{d\rho^2} - (\frac{1}{4}-\frac{2Z}{\rho k})u_l(\rho) - l(l+1)\frac{u_l(\rho)}{\rho^2} = 0
    \end{gather}


    The question presents the substitution $u_l(\rho)=\rho^{l+1}\exp{-\rho/2}\omega(\rho)$, which forms\dots

    \begin{gather}
        \frac{d^2}{d\rho^2}[\rho^{l+1}\exp{-\rho/2}\omega(\rho)] - (\frac{1}{4}-\frac{2Z}{\rho k})(\rho^{l+1}\exp{-\rho/2}\omega(\rho))
        - l(l+1)\rho^{l-1}\exp{-\rho/2}\omega(\rho) = 0
    \end{gather}
    \medskip
    
    {\centering
    \begin{gather*}
        (l+1)[(l\rho^{l-1}\exp{-\rho/2}-\frac{1}{2}\rho^{l+1}\exp{-\rho/2})\omega(\rho) + \rho^l \exp{-\rho/2}\frac{d\omega(\rho)}{d\rho}]\\
        - \frac{1}{2}\{  [(l+1) \rho^l \exp{-\rho/2} 
        - \frac{1}{2}\rho^{l+1}\exp{-\rho/2}]\omega(\rho) 
        + \frac{d\omega(\rho)}{d\rho^2}\rho^{l+1}\exp{-\rho/2}\}\\ 
        +[(l+1)\rho^l\exp{-\rho/2}-\frac{1}{2}\rho^{l+1}\exp{-\rho/2}]\frac{d\omega(\rho)}{d\rho} + \frac{d^2\omega(\rho)}{d\rho^2}\rho^{l+1}\exp{-\rho/2}\\
        - (\frac{1}{4}-\frac{2Z}{k\rho})\rho^{l+1}\exp{-\rho/2}\omega(\rho) - l(l+1)\rho^{l-1}\exp{-\rho/2}\omega(\rho)
        = 0
    \end{gather*}
    }

    and simplifies to

    \begin{gather}
        \frac{d^2\omega(\rho)}{d\rho^2}\rho^{l+1} + \frac{d\omega(\rho)}{d\rho}[2(l+1)\rho^l - \rho^{l+1}] - \omega(\rho)[(l+1)\rho^l - \frac{2Z}{k}\rho^l]
        =0
    \end{gather}

    We now eliminate $\rho^l$ on all terms to get:

    \begin{gather}
        \frac{d^2\omega(\rho)}{d\rho^2}\rho + [2(l+1) - \rho]\frac{d\omega(\rho)}{d\rho} - [(l+1) - \frac{2Z}{k}]\omega(\rho)
        =0
    \end{gather}
    
    This differential equation has the form:

    \begin{gather}
        z\frac{d^2w}{dz^2} + (b-z)\frac{dw}{dz} - aw = 0
    \end{gather}

    Which has solutions in the confluent hypergeometric function;

    \begin{gather}
        F(a,b;\rho) = 1 + \frac{a}{b}\frac{\rho}{1!} + \frac{a}{b}\frac{(a+1)}{(b+1)}\frac{\rho^2}{2!} + \dots
    \end{gather}
    
    In this case, the function will truncate so long as $a=1-n$ for $n=1,2,3$,
    in this way, after the $n+1$ term of the series and all subsequent terms must simplify to zero.

    By comparing the equation we have with the general form, we can see that

    \begin{align}
        a &= l+1 - \frac{2Z}{k}\\
        b &= 2(l+1)
    \end{align}

    And knowing that the differential equation has a general solution in the form of the hypergeometric functions
    and that the series truncates to be a finite sum, we know that this set of equations 
    satisfies the conditions for a solution of $\omega(\rho)$ for bound states of the hydrogen atom.



\section{Question 2}

    The equation:

    \begin{gather}
        F(a,b;\rho) = 1 + \frac{a}{b}\frac{\rho}{1!} + \frac{a}{b}\frac{(a+1)}{(b+1)}\frac{\rho^2}{2!} + \dots
    \end{gather}

    Terminates for $a = 1 - n$, for $n \in \{1,2,3,\dots\}$. 
    This prevents the series from growing exponentially in $\rho$.\\

    In our case, we have $a = 1 + l - \frac{2Z}{k}$, which can be rewritten as $a = 1 - (\frac{2Z}{k}-l)$.\\
    This makes our $n = \frac{2Z}{k}-l$ and subsequently $n+l=\frac{2Z}{k}$.\\ 
    \smallskip
    We then write $n=\frac{2Z}{k}, \;\forall\; n \in \{1 + l, 2 + l, 3 + l, \dots$\}.\\

\section{Question 3}

    2.28 states:

    \begin{gather}
        \int_{0}^{\infty}dr u_{n'l}(r) u_{nl}(r) = \delta_{n'n}
    \end{gather}
    
    Which tell us that the eigenstates are orthogonal and normalised for $n=n'$, where the kronecker delta equals unity.
    This will allow us to calculate the normalisation coefficients for our wave-functions, $u_{21}(r)$ and $u_{31}(r)$.\medskip

    For $\mathbf{u_{21}(r)}$;\smallskip

    First we establish what we are substituting for $\rho$, with $Z=1,\; n=2, \; l=1$:

    \begin{gather*}
        \rho = kr = \frac{2Zr}{n}\\
        \rho = kr = \frac{2(1)r}{2} = r\\
    \end{gather*}\vspace{-1.5cm}
    \begin{gather}
        \therefore k = 1
    \end{gather}
    

    With $l=1=Z=k=1$ we have:
    
    \begin{gather*} 
             a = l + 1 - \frac{2Z}{k}\\
             a = 1 + 1 - 2 = 0\\
             b = 2(l+1)\\
             b= 2(2) = 4
    \end{gather*}\vspace{-1.5cm}
    \begin{gather}
        a = 0, \; b= 4
    \end{gather}

    
    Calculating the $\omega(kr)$
    \begin{gather*}
        F(a,b;r) = 1 + \frac{a}{b}\frac{r}{1!} + \frac{a}{b}\frac{(a+1)}{(b+1)}\frac{r^2}{2!} + \dots\\
        F(0,4;r) = 1 + \frac{0}{4}\frac{r}{1!} + \frac{0}{4}\frac{(0+1)}{(4+1)}\frac{r^2}{2!} + \dots\\
    \end{gather*}\vspace{-1.5cm}
    \begin{gather}
        F(0,4;r) = \omega(r)=1 
    \end{gather}


    
    
    Substituting $r$ for $\rho$ to get back $u_{nl}(r)$ from $u_{nl}(\rho)$:\medskip



    \begin{gather*}
        u_{nl}(r) = (kr)^{l+1}\exp{-kr/2}\omega(kr)\\
        u_{21}(r) = r^{1+1}\exp{-r/2}(1)
    \end{gather*}
    \begin{gather}
        u_{21}(r) = r^{2}\exp{-r/2}
    \end{gather}

    We need to add a constant of normalisation to this function in order for it to belong to the Hilbert space,
    and we will use (13) in order to normalise.

    \begin{gather*}
        \int_{0}^{\infty} (Ar^{2}\exp{-r/2})^2dr = \delta_{n'n}\\
        \int_{0}^{\infty} A^2r^{4}\exp{-r}dr = \delta_{2,2} = 1\\
    \end{gather*}

    Tabular integration will solve the integral

    \begin{table}[h]
        \centering
        \begin{tabular}{cc}
        \hline
        \multicolumn{1}{|c|}{F(x)} & \multicolumn{1}{c|}{G(x)} \\ \hline
                 &  \\ 
         $r^4$   & $e^{-r}$ \\
         $-4r^3$  & $-e^{-r}$ \\
         $12r^2$ & $e^{-r}$ \\
         $-24r$ & $-e^{-r}$ \\
         $24$    & $e^{-r}$ \\
         $0$     & $-e^{-r}$ \\
                 & $e^{-r}$ \\ \hline
        \end{tabular}
    \end{table}

    \begin{gather*}
        \int_{0}^{\infty} A^2r^{4}\exp{-r}dr  \\
        = A^2[-r^4\exp{-r} - 4r^3\exp{-r} - 12r^2\exp{-r} - 24r\exp{-r} -24\exp{-r}]^{\infty}_{0}\\
        = A^2[0 - (-24)]\\
        = 24A^2 = 1\\
    \end{gather*}\vspace{-1.5cm}
    \begin{gather} 
        A = \frac{1}{2\sqrt{6}} 
    \end{gather}
        
    

    Which normalises the function to

    \begin{gather}
        u_{21}(r) = \frac{r^2}{2\sqrt{6}}\exp{-r/2}
    \end{gather}

    as given in the problem statement.

    \medskip

    For $\mathbf{u_{31}(r)}$:

    We start in the same way, by defining the appropriate quantities starting with $Z=1,\; n=3, \; l=1$.
    Subsequently computing parameters like k:

    \begin{gather*}
        \rho = kr = \frac{2Zr}{n}\\
        \rho = kr = \frac{2(1)r}{3} = r\\
    \end{gather*}\vspace{-1.5cm}
    \begin{gather}
        \therefore k = \frac{2}{3}
    \end{gather}

    $a$ and $b$\dots

    \begin{gather*} 
        a = l + 1 - \frac{2Z}{k}\\
        a = 1 + 1 - \frac{2(1)}{\frac{2}{3}}\\
        a = 1 + 1 - 3 = -1\\
        b = 2(l+1)\\
        b= 2(2) = 4
    \end{gather*}\vspace{-0.5cm}
    \begin{gather}
    a = -1, \; b= 4
    \end{gather}

    Taking these values we compute the $\omega(\rho)$ value needed for the function.

    \begin{gather*}
        F(a,b;\rho) = 1 + \frac{a}{b}\frac{\rho}{1!} + \frac{a}{b}\frac{(a+1)}{(b+1)}\frac{\rho^2}{2!} + \dots\\
        F(-1,4;\rho) = 1 + \frac{-1}{4}\frac{\rho}{1!} + \frac{-1}{4}\frac{(-1+1)}{(4+1)}\frac{\rho^2}{2!} + \dots\\
    \end{gather*}\vspace{-1.5cm}
    \begin{gather}
        F(-1,4;\rho) = 1 - \frac{\rho}{4} 
    \end{gather}

    Replacing $\rho$ with $\frac{2}{3}r$

    \begin{gather}
        \omega(\frac{2}{3}r) = F(-1,4;\frac{2}{3}r) = 1 - \frac{1}{4}\frac{2}{3}r \\
        \omega(\frac{2}{3}r) = 1 - \frac{r}{6}
    \end{gather}

    We now make the appropriate substitutions as follows:

    \begin{gather*}
        u_{nl}(r) = (kr)^{l+1}\exp{-kr/2}\omega(kr)\\
        u_{31}(r) = (\frac{2}{3}r)^{1+1}\exp{-\frac{r}{2}\frac{2}{3}}(1-\frac{r}{6})\\
        u_{31}(r) = (\frac{4}{9})r^2\exp{-\frac{r}{3}}(1-\frac{r}{6})
    \end{gather*}
    
    And add the necessary normalisation coefficient $A$:

    \begin{gather}
        u_{31}(r) = A(\frac{4}{9})r^2\exp{-\frac{r}{3}}(1-\frac{r}{6})
    \end{gather}

    As last time we now use the normalisation condition of Equation 13 to determine the normalisation coefficient

    \begin{gather*}
        \int_{0}^{\infty}dr u_{n'l}(r) u_{nl}(r) = \delta_{n'n}\\
        \int_{0}^{\infty} (A(\frac{4}{9})r^2\exp{-\frac{r}{3}}(1-\frac{r}{6}))^2dr = \delta_{3'3}\\
        \int_{0}^{\infty} A^2(\frac{16}{81})\exp{-\frac{2r}{3}}(r^4 - \frac{r^5}{3}+\frac{r^6}{36})dr = \delta_{3,3} = 1
    \end{gather*}
    \begin{gather}
        A^2(\frac{16}{81})\int_{0}^{\infty} \exp{-\frac{2r}{3}}(r^4 - \frac{r^5}{3}+\frac{r^6}{36})dr  = 1
    \end{gather}

    As before, the form of integral we have is an exponent multiplied by a polynomial, so we know that tabular integration
    will solve the integral:

    \begin{table}[h]
        \centering
        \begin{tabular}{cc}
        \hline
        \multicolumn{1}{|c|}{F(x)} & \multicolumn{1}{c|}{G(x)} \\ \hline
                 &  \\ 
         $r^4 - \frac{r^5}{3}+\frac{r^6}{36}$   & $\exp{-\frac{2r}{3}}$ \\
         &  \\
         $-(4r^3 - \frac{5}{3}r^4 + \frac{6}{36}r^5)$  & $-\frac{3}{2}\exp{-\frac{2r}{3}}$ \\
         &  \\
         $12r^2 - \frac{20}{3}r^3 + \frac{5}{6}r^4$ & $\frac{9}{4}\exp{-\frac{2r}{3}}$ \\
         &  \\
         $-(24r - 20r^2 + \frac{20}{6}r^3)$ & $-\frac{27}{8}\exp{-\frac{2r}{3}}$ \\
         &  \\
         $24 - 40r + 10r^2$    & $\frac{81}{16}\exp{-\frac{2r}{3}}$ \\
         &  \\
         $-(-40 + 20r)$     & $-\frac{243}{32}\exp{-\frac{2r}{3}}$ \\
         &  \\
         $20$       & $\frac{729}{64}\exp{-\frac{2r}{3}}$ \\\
         &  \\ 
         $0$     & $-\frac{2187}{128}\exp{-\frac{2r}{3}}$    \\       \hline
        \end{tabular}
    \end{table}

    Resulting in the final integral

    \begin{gather*}
        A^2(\frac{16}{81})\int_{0}^{\infty} \exp{-\frac{2r}{3}}(r^4 - \frac{r^5}{3}+\frac{r^6}{36})dr  \\
        = A^2(\frac{16}{81})
        [   
        -\frac{3}{2}\exp{-\frac{2r}{3}}(r^4 - \frac{r^5}{3}+\frac{r^6}{36})
        -\frac{9}{4}\exp{-\frac{2r}{3}}(4r^3 - \frac{5}{3}r^4 + \frac{6}{36}r^5)\\
        -\frac{27}{8}\exp{-\frac{2r}{3}}(12r^2 - \frac{20}{3}r^3 + \frac{5}{6}r^4)
        -\frac{81}{16}\exp{-\frac{2r}{3}}(24r - 20r^2 + \frac{20}{6}r^3)\\
        -\frac{243}{32}\exp{-\frac{2r}{3}}(24 - 40r + 10r^2)
        -\frac{729}{64}\exp{-\frac{2r}{3}}(-40 + 20r)
        -20\frac{2187}{128}\exp{-\frac{2r}{3}}]^{\infty}_{0}=1\\
    \end{gather*}

    Which in the limits of the integration will evaluate to:

    \begin{gather*}
        = A^2(\frac{16}{81})(\frac{2187}{32})=1\\
        = \frac{27}{2}A^2 = 1
    \end{gather*}
    \begin{gather}
        A = \frac{2}{3\sqrt{6}}
    \end{gather}
        
    

    When finally substituted into the function for $u$:

    \begin{gather}
        u_{31}(r) = \frac{2}{3\sqrt{6}}(\frac{4}{9})r^2\exp{-\frac{r}{3}}(1-\frac{r}{6})\\
        u_{31}(r) = \frac{8r^2}{27\sqrt{6}}\exp{-\frac{r}{3}}(1-\frac{r}{6})
    \end{gather}






\end{document}